Change iterate's _ .. _ notation to { _ .. _ }
In the grammar, the .. operator is no longer an infix, but part of a
"close-fix" notation involving the braces.  This is the same as the way
listRange sets up its [ m .. n ] syntax.

Most (but not all) uses end up needing to parenthesise, e.g., in
things like

  sum (m .. n)

so changing to braces doesn't waste characters.

Note that this notion has nothing to do with real numbers, so I will
work towards moving it into pred_set at some future date.  There are
also lots of theorems about it that should be automatic.

src/probability/real_topologyScript.sml
@@ -333,13 +333,13 @@ val LINEAR_SUM_MUL = store_thm ("LINEAR_SUM_MUL",
   SIMP_TAC std_ss [LINEAR_SUM, o_DEF, LINEAR_CMUL]);
 
 val lemma = prove (
- ``x = sum (1:num..1:num) (\i. x * &i)``,
+ ``x = sum {1..1} (\i. x * &i)``,
   REWRITE_TAC [SUM_SING_NUMSEG] THEN BETA_TAC THEN REAL_ARITH_TAC);
 
 val LINEAR_BOUNDED = store_thm ("LINEAR_BOUNDED",
  ``!f:real->real. linear f ==> ?B. !x. abs(f x) <= B * abs(x)``,
   REPEAT STRIP_TAC THEN EXISTS_TAC
-   ``sum(1:num..1:num) (\i. abs((f:real->real)(&i)))`` THEN
+   ``sum{1:num..1:num} (\i. abs((f:real->real)(&i)))`` THEN
   GEN_TAC THEN
   GEN_REWR_TAC (LAND_CONV o funpow 2 RAND_CONV) [lemma] THEN
   ASM_SIMP_TAC std_ss [LINEAR_SUM, FINITE_NUMSEG] THEN
@@ -443,14 +443,14 @@ val BILINEAR_SUM = store_thm ("BILINEAR_SUM",
   SIMP_TAC std_ss [lemma]);
 
 val lemma = prove (
- ``!x. x = sum (1:num..1:num) (\i. x * &i)``,
+ ``!x. x = sum {1:num..1:num} (\i. x * &i)``,
   REWRITE_TAC [SUM_SING_NUMSEG] THEN BETA_TAC THEN REAL_ARITH_TAC);
 
 val BILINEAR_BOUNDED = store_thm ("BILINEAR_BOUNDED",
  ``!h:real->real->real.
         bilinear h ==> ?B. !x y. abs(h x y) <= B * abs(x) * abs(y)``,
   REPEAT STRIP_TAC THEN
-  EXISTS_TAC ``sum ((1:num..1:num) CROSS (1:num..1:num))
+  EXISTS_TAC ``sum ({1:num..1:num} CROSS {1:num..1:num})
                   (\ (i,j). abs((h:real->real->real)
                                 (&i) (&j)))`` THEN
   REPEAT GEN_TAC THEN GEN_REWR_TAC
@@ -479,9 +479,9 @@ val BILINEAR_BOUNDED_POS = store_thm ("BILINEAR_BOUNDED_POS",
 val BILINEAR_SUM_PARTIAL_SUC = store_thm ("BILINEAR_SUM_PARTIAL_SUC",
  ``!f g h:real->real->real m n.
         bilinear h
-        ==> (sum (m..n) (\k. h (f k) (g(k + 1) - g(k))) =
+        ==> (sum {m..n} (\k. h (f k) (g(k + 1) - g(k))) =
                 if m <= n then h (f(n + 1)) (g(n + 1)) - h (f m) (g m) -
-                               sum (m..n) (\k. h (f(k + 1) - f(k)) (g(k + 1)))
+                               sum {m..n} (\k. h (f(k + 1) - f(k)) (g(k + 1)))
                 else 0)``,
   SIMP_TAC std_ss [RIGHT_FORALL_IMP_THM] THEN REPEAT GEN_TAC THEN DISCH_TAC THEN
   GEN_TAC THEN INDUCT_TAC THEN
@@ -504,9 +504,9 @@ val BILINEAR_SUM_PARTIAL_SUC = store_thm ("BILINEAR_SUM_PARTIAL_SUC",
 val BILINEAR_SUM_PARTIAL_PRE = store_thm ("BILINEAR_SUM_PARTIAL_PRE",
  ``!f g h:real->real->real m n.
         bilinear h
-        ==> (sum (m..n) (\k. h (f k) (g(k) - g(k - 1))) =
+        ==> (sum {m..n} (\k. h (f k) (g(k) - g(k - 1))) =
                 if m <= n then h (f(n + 1)) (g(n)) - h (f m) (g(m - 1)) -
-                               sum (m..n) (\k. h (f(k + 1) - f(k)) (g(k)))
+                               sum {m..n} (\k. h (f(k + 1) - f(k)) (g(k)))
                 else 0)``,
   REPEAT STRIP_TAC THEN
   FIRST_ASSUM(MP_TAC o ISPECL [``f:num->real``, ``\k. (g:num->real)(k - 1)``,
@@ -1487,7 +1487,7 @@ val MAXIMAL_INDEPENDENT_SUBSET_EXTEND = store_thm ("MAXIMAL_INDEPENDENT_SUBSET_E
  ``!s v:real->bool. s SUBSET v /\ independent s ==> ?b. s SUBSET b /\ b SUBSET v /\
    independent b /\ v SUBSET (span b)``,
   REPEAT GEN_TAC THEN
-  completeInduct_on `(1:num) - CARD(s:real->bool)` THEN
+  completeInduct_on ` 1n - CARD(s:real->bool)` THEN
   GEN_TAC THEN DISCH_TAC THEN FULL_SIMP_TAC std_ss [] THEN POP_ASSUM K_TAC THEN
   REPEAT STRIP_TAC THEN
   ASM_CASES_TAC ``v SUBSET (span(s:real->bool))`` THENL
@@ -1495,8 +1495,8 @@ val MAXIMAL_INDEPENDENT_SUBSET_EXTEND = store_thm ("MAXIMAL_INDEPENDENT_SUBSET_E
   FIRST_X_ASSUM(MP_TAC o REWRITE_RULE [SUBSET_DEF]) THEN
   SIMP_TAC std_ss [NOT_FORALL_THM, NOT_IMP] THEN
   DISCH_THEN(X_CHOOSE_THEN ``a:real`` STRIP_ASSUME_TAC) THEN
-  KNOW_TAC ``(!(m :num). m < (1 :num) - CARD (s :real -> bool) ==>
-        !(s :real -> bool). (m = (1 :num) - CARD s) ==>
+  KNOW_TAC ``(!(m :num). m <  1n - CARD (s :real -> bool) ==>
+        !(s :real -> bool). (m =  1n - CARD s) ==>
           s SUBSET (v :real -> bool) /\ independent s ==>
           ?(b :real -> bool).
             s SUBSET b /\ b SUBSET v /\ independent b /\ v SUBSET span b) ==>
@@ -1982,7 +1982,7 @@ val DIM_SUBSET = store_thm ("DIM_SUBSET",
   MESON_TAC[BASIS_EXISTS, INDEPENDENT_SPAN_BOUND, SUBSET_DEF, HAS_SIZE]);
 
 val DIM_SUBSET_UNIV = store_thm ("DIM_SUBSET_UNIV",
- ``!s:real->bool. dim(s) <= (1:num)``,
+ ``!s:real->bool. dim(s) <=  1n``,
   GEN_TAC THEN REWRITE_TAC[GSYM DIM_UNIV] THEN
   MATCH_MP_TAC DIM_SUBSET THEN REWRITE_TAC[SUBSET_UNIV]);
 
@@ -7409,7 +7409,7 @@ val CAUCHY_IMP_BOUNDED = store_thm ("CAUCHY_IMP_BOUNDED",
   ASSUME_TAC THENL
    [ASM_MESON_TAC[GREATER_EQ, dist, DIST_SYM, ABS_TRIANGLE_SUB,
                   REAL_ARITH ``a <= b + c /\ c < &1 ==> a <= b + &1:real``],
-    MP_TAC(ISPECL [``\n:num. abs(s n :real)``, ``0..N``]
+    MP_TAC(ISPECL [``\n:num. abs(s n :real)``, ``{0..N}``]
                   UPPER_BOUND_FINITE_SET_REAL) THEN
     SIMP_TAC std_ss [FINITE_NUMSEG, IN_NUMSEG, LESS_EQ_0, GSYM LEFT_EXISTS_IMP_THM] THEN
     ASM_MESON_TAC[LESS_EQ_CASES,
@@ -7701,7 +7701,7 @@ val LIMPT_OF_SEQUENCE_SUBSEQUENCE = store_thm ("LIMPT_OF_SEQUENCE_SUBSEQUENCE",
   FIRST_ASSUM(MP_TAC o REWRITE_RULE [LIMPT_APPROACHABLE]) THEN
   DISCH_THEN(MP_TAC o GEN ``n:num`` o SPEC
    ``inf((inv(&n + &1:real)) INSERT IMAGE (\k. dist((f:num->real) k,l))
-         {k | k IN (0:num)..n /\ ~(f k = l)})``) THEN
+         {k | k IN {0..n} /\ ~(f k = l)})``) THEN
   SIMP_TAC std_ss [REAL_LT_INF_FINITE, FINITE_INSERT, NOT_INSERT_EMPTY,
    FINITE_RESTRICT, FINITE_NUMSEG, IMAGE_FINITE] THEN
   SIMP_TAC std_ss [FORALL_IN_INSERT, EXISTS_IN_IMAGE, FORALL_IN_IMAGE, IN_UNIV] THEN
@@ -8181,11 +8181,11 @@ val BOUNDED_CLOSED_NEST = store_thm ("BOUNDED_CLOSED_NEST",
   DISCH_THEN(CONJUNCTS_THEN2 ASSUME_TAC MP_TAC) THEN
   DISCH_THEN(CONJUNCTS_THEN2
      (X_CHOOSE_TAC ``a:num->real``) STRIP_ASSUME_TAC) THEN
-  SUBGOAL_THEN ``compact(s (0:num):real->bool)`` MP_TAC THENL
+  SUBGOAL_THEN ``compact(s  0n:real->bool)`` MP_TAC THENL
    [METIS_TAC[BOUNDED_CLOSED_IMP_COMPACT], ALL_TAC] THEN
   REWRITE_TAC[compact] THEN
   DISCH_THEN(MP_TAC o SPEC ``a:num->real``) THEN
-  KNOW_TAC ``(!n:num. a n IN s (0:num):real->bool)`` THENL
+  KNOW_TAC ``(!n:num. a n IN s  0n:real->bool)`` THENL
   [ASM_MESON_TAC[SUBSET_DEF, ZERO_LESS_EQ],
    DISCH_TAC THEN ASM_REWRITE_TAC []] THEN
   DISCH_THEN (X_CHOOSE_TAC ``l:real``) THEN
@@ -11168,13 +11168,13 @@ val CAUCHY_CONTINUOUS_UNIQUENESS_LEMMA = store_thm
         m >= N /\ n >= N ==>
         (dist
            ((\(n :num).
-               if EVEN n then (x :num -> real) (n DIV (2 :num))
-               else (y :num -> real) (n DIV (2 :num))) m,
+               if EVEN n then (x :num -> real) (n DIV  2n)
+               else (y :num -> real) (n DIV  2n)) m,
             (\(n :num).
-               if EVEN n then x (n DIV (2 :num))
-               else y (n DIV (2 :num))) n) :real) < e) /\
+               if EVEN n then x (n DIV  2n)
+               else y (n DIV  2n)) n) :real) < e) /\
       (!(n :num). (\(n :num).
-       if EVEN n then x (n DIV (2 :num)) else y (n DIV (2 :num))) n IN
+       if EVEN n then x (n DIV  2n) else y (n DIV  2n)) n IN
     (s :real -> bool))`` THENL
   [ (* goal 1 (of 2) *)
     CONJ_TAC THENL [ALL_TAC, METIS_TAC[]] THEN
@@ -13556,7 +13556,7 @@ val OPEN_UNION_COMPACT_SUBSETS = store_thm ("OPEN_UNION_COMPACT_SUBSETS",
   KNOW_TAC ``?(f :num -> real -> bool).
            (\f. !(n :num). compact (f n)) f /\
            (\f. !(n :num). f n SUBSET (s :real -> bool)) f /\
-           (\f. !(n :num). f n SUBSET interior (f (n + (1 :num)))) f /\
+           (\f. !(n :num). f n SUBSET interior (f (n +  1n))) f /\
            (\f. BIGUNION {f n | n IN univ((:num) :num itself)} = s) f /\
   (\f. !(k :real -> bool).
     compact k /\ k SUBSET s ==>
@@ -14130,16 +14130,16 @@ val UNIT_INTERVAL_NONEMPTY = store_thm ("UNIT_INTERVAL_NONEMPTY",
 val IMAGE_STRETCH_INTERVAL = store_thm
   ("IMAGE_STRETCH_INTERVAL",
  ``!a b:real m.
-    IMAGE (\x. @f. f = m(1:num) * x) (interval[a,b]) =
+    IMAGE (\x. @f. f = m 1n * x) (interval[a,b]) =
         if interval[a,b] = {} then {}
-        else interval[(@f. f = min (m(1:num) * a) (m(1:num) * b)):real,
-                      (@f. f = max (m(1:num) * a) (m(1:num) * b))]``,
+        else interval[(@f. f = min (m 1n * a) (m 1n * b)):real,
+                      (@f. f = max (m 1n * a) (m 1n * b))]``,
   REPEAT GEN_TAC THEN COND_CASES_TAC THEN ASM_SIMP_TAC std_ss [IMAGE_EMPTY, IMAGE_INSERT] THEN
   ASM_SIMP_TAC std_ss [EXTENSION, IN_IMAGE, IN_INTERVAL, GSYM FORALL_AND_THM,
                TAUT `(a ==> b) /\ (a ==> c) <=> a ==> b /\ c`] THEN
   X_GEN_TAC ``x:real`` THEN
   FIRST_X_ASSUM(MP_TAC o REWRITE_RULE [INTERVAL_NE_EMPTY]) THEN
-  ASM_CASES_TAC ``(m:num->real) (1:num) = &0`` THENL
+  ASM_CASES_TAC ``(m:num->real)  1n = &0`` THENL
    [ASM_SIMP_TAC std_ss [REAL_MUL_LZERO, REAL_MAX_ACI, REAL_MIN_ACI] THEN
     METIS_TAC[REAL_LE_ANTISYM, REAL_LE_REFL],
     ALL_TAC] THEN
@@ -14179,7 +14179,7 @@ val IMAGE_STRETCH_INTERVAL = store_thm
 
 val INTERVAL_IMAGE_STRETCH_INTERVAL = store_thm ("INTERVAL_IMAGE_STRETCH_INTERVAL",
  ``!a b:real m. ?u v:real.
-     IMAGE (\x. @f. f = m (1:num) * x) (interval[a,b]) = interval[u,v]``,
+     IMAGE (\x. @f. f = m  1n * x) (interval[a,b]) = interval[u,v]``,
   SIMP_TAC std_ss [IMAGE_STRETCH_INTERVAL] THEN METIS_TAC[EMPTY_AS_INTERVAL]);
 
 val CLOSED_INTERVAL_IMAGE_UNIT_INTERVAL = store_thm ("CLOSED_INTERVAL_IMAGE_UNIT_INTERVAL",
@@ -14190,7 +14190,7 @@ val CLOSED_INTERVAL_IMAGE_UNIT_INTERVAL = store_thm ("CLOSED_INTERVAL_IMAGE_UNIT
                                          (interval[0:real,1])))``,
   REWRITE_TAC[INTERVAL_NE_EMPTY] THEN REPEAT STRIP_TAC THEN
   ONCE_REWRITE_TAC [METIS [] ``(\x. @f. f = (b - a) * x) =
-                               (\x. @f. f = (\x. (b - a)) (1:num) * x:real)``] THEN
+                               (\x. @f. f = (\x. (b - a))  1n * x:real)``] THEN
   REWRITE_TAC[IMAGE_STRETCH_INTERVAL] THEN
   SIMP_TAC std_ss [REAL_MUL_RZERO, REAL_MUL_RID, UNIT_INTERVAL_NONEMPTY] THEN
   REWRITE_TAC[EXTENSION, IN_INTERVAL] THEN
@@ -16255,10 +16255,10 @@ val HOMEOMORPHIC_OPEN_INTERVAL_UNIV = store_thm ("HOMEOMORPHIC_OPEN_INTERVAL_UNI
 (* ------------------------------------------------------------------------- *)
 
 Triviality lemma:
-  !s m n. sum (s INTER (m..n)) (\i. inv(&3 pow i)) < &3 / &2 / &3 pow m
+  !s m n. sum (s INTER {m..n}) (\i. inv(&3 pow i)) < &3 / &2 / &3 pow m
 Proof
     REPEAT GEN_TAC THEN MATCH_MP_TAC REAL_LET_TRANS THEN
-    EXISTS_TAC ``sum (m..n) (\i. inv(&3 pow i))`` THEN CONJ_TAC THENL
+    EXISTS_TAC ``sum {m..n} (\i. inv(&3 pow i))`` THEN CONJ_TAC THENL
     [ (* goal 1 (of 2) *)
       MATCH_MP_TAC SUM_SUBSET_SIMPLE THEN
       SIMP_TAC std_ss [FINITE_NUMSEG, INTER_SUBSET, REAL_LE_INV_EQ,
@@ -16268,9 +16268,9 @@ Proof
       DISCH_TAC THEN FULL_SIMP_TAC std_ss [] THEN POP_ASSUM K_TAC THEN
       KNOW_TAC ``(!m'. m' < n - m ==>
         !n m''. (m' = n - m'') ==>
-          sum (m'' .. n) (\i. inv (3 pow i)) < 3 / 2 / 3 pow m'') ==>
+          sum {m'' .. n} (\i. inv (3 pow i)) < 3 / 2 / 3 pow m'') ==>
        (!n' m''. (n' - m'' < n - m) ==>
-          sum (m'' .. n') (\i. inv (3 pow i)) < 3 / 2 / 3 pow m'')`` THENL
+          sum {m'' .. n'} (\i. inv (3 pow i)) < 3 / 2 / 3 pow m'')`` THENL
       [ METIS_TAC [], ASM_REWRITE_TAC [] THEN POP_ASSUM K_TAC THEN DISCH_TAC ] THEN
       ASM_CASES_TAC ``m:num <= n`` THENL
       [ (* goal 2.1 (of 2) *)
@@ -16369,7 +16369,7 @@ Proof
 
     (* goal 2 (of 2) *)
     REWRITE_TAC[le_c, IN_UNIV] THEN
-    EXISTS_TAC ``\s:num->bool. sup { sum (s INTER ((0:num)..n)) (\i. inv(&3 pow i)) |
+    EXISTS_TAC ``\s:num->bool. sup { sum (s INTER { 0n..n}) (\i. inv(&3 pow i)) |
                                     n IN univ(:num) }`` THEN
     MAP_EVERY X_GEN_TAC [``x:num->bool``, ``y:num->bool``] THEN
     ONCE_REWRITE_TAC[MONO_NOT_EQ] THEN
@@ -16380,8 +16380,8 @@ Proof
     MAP_EVERY (fn w => SPEC_TAC(w,w)) [``y:num->bool``, ``x:num->bool``] THEN
     KNOW_TAC ``!x y.
      (?n. ~(n IN x <=> n IN y) /\ (\x y n. !m. m < n ==> (m IN x <=> m IN y)) x y n) ==>
-     (\x y. sup {sum (x INTER (0 .. n)) (\i. inv (3 pow i)) | n IN univ(:num)} <>
-            sup {sum (y INTER (0 .. n)) (\i. inv (3 pow i)) | n IN univ(:num)}) x y`` THENL
+     (\x y. sup {sum (x INTER {0 .. n}) (\i. inv (3 pow i)) | n IN univ(:num)} <>
+            sup {sum (y INTER {0 .. n}) (\i. inv (3 pow i)) | n IN univ(:num)}) x y`` THENL
     [ALL_TAC, METIS_TAC []] THEN
     MATCH_MP_TAC(MESON[]
      ``((!P Q n. R P Q n <=> R Q P n) /\ (!P Q. SS P Q <=> SS Q P)) /\
@@ -16393,11 +16393,11 @@ Proof
     DISCH_THEN(X_CHOOSE_THEN ``n:num`` STRIP_ASSUME_TAC) THEN
     MATCH_MP_TAC(REAL_ARITH ``!z:real. y < z /\ z <= x ==> ~(x = y)``) THEN
 
-    EXISTS_TAC ``sum (x INTER ((0:num)..n)) (\i. inv(&3 pow i))`` THEN CONJ_TAC THENL
+    EXISTS_TAC ``sum (x INTER { 0n..n}) (\i. inv(&3 pow i))`` THEN CONJ_TAC THENL
     [ (* goal 2.1 (of 2) *)
       MATCH_MP_TAC REAL_LET_TRANS THEN
       EXISTS_TAC
-       ``sum (y INTER ((0:num)..n)) (\i. inv(&3 pow i)) +
+       ``sum (y INTER { 0n..n}) (\i. inv(&3 pow i)) +
          &3 / &2 / &3 pow (SUC n)`` THEN
 
       CONJ_TAC THENL
@@ -16406,7 +16406,7 @@ Proof
         X_GEN_TAC ``p:num`` THEN ASM_CASES_TAC ``n:num <= p`` THENL
          [MATCH_MP_TAC(REAL_ARITH
            ``!d. (s:real = t + d) /\ d <= e ==> s <= t + e``) THEN
-          EXISTS_TAC ``sum(y INTER (n+(1:num)..p)) (\i. inv (&3 pow i))`` THEN
+          EXISTS_TAC ``sum(y INTER {n+ 1n..p}) (\i. inv (&3 pow i))`` THEN
           CONJ_TAC THENL
            [ONCE_REWRITE_TAC[INTER_COMM] THEN
             SIMP_TAC std_ss [INTER_DEF, SUM_RESTRICT_SET] THEN
@@ -16440,10 +16440,10 @@ Proof
             ONCE_REWRITE_TAC [REAL_MUL_SYM] THEN
             SIMP_TAC real_ss [REAL_MUL_ASSOC, REAL_MUL_LINV] THEN
             SIMP_TAC real_ss [REAL_INV_1OVER, REAL_LT_LDIV_EQ]]]],
-      MP_TAC(ISPEC ``{ sum (x INTER ((0:num)..n)) (\i. inv(&3 pow i)) | n IN univ(:num) }``
+      MP_TAC(ISPEC ``{ sum (x INTER { 0n..n}) (\i. inv(&3 pow i)) | n IN univ(:num) }``
           SUP) THEN SIMP_TAC std_ss [FORALL_IN_GSPEC, IN_UNIV] THEN
-      KNOW_TAC ``{sum (x INTER (0 .. n)) (\i. inv (3 pow i)) | n | T} <> {} /\
-         (?b. !n. sum (x INTER (0 .. n)) (\i. inv (3 pow i)) <= b)`` THENL
+      KNOW_TAC ``{sum (x INTER {0 .. n}) (\i. inv (3 pow i)) | n | T} <> {} /\
+         (?b. !n. sum (x INTER {0 .. n}) (\i. inv (3 pow i)) <= b)`` THENL
       [ALL_TAC, DISCH_TAC THEN ASM_REWRITE_TAC [] THEN POP_ASSUM K_TAC THEN
        SIMP_TAC std_ss []] THEN
       CONJ_TAC THENL [SET_TAC[], ALL_TAC] THEN
@@ -16962,7 +16962,7 @@ val OPEN_SURJECTIVE_LINEAR_IMAGE = store_thm ("OPEN_SURJECTIVE_LINEAR_IMAGE",
   FIRST_ASSUM(MP_TAC o GEN ``k:num`` o SPEC ``if (1 = k:num) then &1 else &0:real``) THEN
   SIMP_TAC std_ss [SKOLEM_THM] THEN
   DISCH_THEN(X_CHOOSE_THEN ``b:num->real`` STRIP_ASSUME_TAC) THEN
-  SUBGOAL_THEN ``bounded(IMAGE (b:num->real) ((1:num)..(1:num)))`` MP_TAC THENL
+  SUBGOAL_THEN ``bounded(IMAGE (b:num->real) { 1n.. 1n})`` MP_TAC THENL
    [SIMP_TAC std_ss [FINITE_IMP_BOUNDED, IMAGE_FINITE, FINITE_NUMSEG], ALL_TAC] THEN
   SIMP_TAC std_ss [BOUNDED_POS, FORALL_IN_IMAGE, IN_NUMSEG] THEN
   DISCH_THEN(X_CHOOSE_THEN ``B:real`` STRIP_ASSUME_TAC) THEN
@@ -16975,7 +16975,7 @@ val OPEN_SURJECTIVE_LINEAR_IMAGE = store_thm ("OPEN_SURJECTIVE_LINEAR_IMAGE",
   ASM_SIMP_TAC real_ss [REAL_LT_DIV, REAL_LT, LE_1] THEN
   X_GEN_TAC ``y:real`` THEN DISCH_TAC THEN REWRITE_TAC[IN_IMAGE] THEN
   ABBREV_TAC ``u = y - (f:real->real) x`` THEN
-  EXISTS_TAC ``x + sum(1 .. 1) (\i. (u:real) * b i):real`` THEN
+  EXISTS_TAC ``x + sum{1 .. 1} (\i. (u:real) * b i):real`` THEN
   ASM_SIMP_TAC std_ss [LINEAR_ADD, LINEAR_SUM, FINITE_NUMSEG, o_DEF,
                LINEAR_CMUL] THEN
   CONJ_TAC THENL [EXPAND_TAC "u" THEN SIMP_TAC std_ss [NUMSEG_SING, SUM_SING] THEN
@@ -17354,7 +17354,7 @@ val _ = hide "summable";
 val _ = set_fixity "sums" (Infix(NONASSOC, 450));
 
 Definition sums : (* cf. seqTheory.sums *)
-   (f sums l) s = ((\n. sum (s INTER ((0:num)..n)) f) --> l) sequentially
+   (f sums l) s = ((\n. sum (s INTER { 0n..n}) f) --> l) sequentially
 End
 
 Definition infsum : (* cf. seqTheory.suminf *)
@@ -17409,18 +17409,18 @@ val SUMS_INFSUM = store_thm ("SUMS_INFSUM",
 
 val SUMS_LIM = store_thm ("SUMS_LIM",
  ``!f:num->real s.
-      (f sums lim sequentially (\n. sum (s INTER ((0:num)..n)) f)) s
+      (f sums lim sequentially (\n. sum (s INTER { 0n..n}) f)) s
       <=> summable s f``,
   GEN_TAC THEN GEN_TAC THEN EQ_TAC THENL [MESON_TAC[summable],
   REWRITE_TAC[summable, sums] THEN STRIP_TAC THEN REWRITE_TAC[lim_def] THEN
   METIS_TAC[]]);
 
 val FINITE_INTER_NUMSEG = store_thm ("FINITE_INTER_NUMSEG",
- ``!s m n. FINITE(s INTER (m..n))``,
+ ``!s m n. FINITE(s INTER {m..n})``,
   MESON_TAC[SUBSET_FINITE_I, FINITE_NUMSEG, INTER_SUBSET]);
 
 val SERIES_FROM = store_thm ("SERIES_FROM",
- ``!f l k. (f sums l) (from k) = ((\n. sum(k..n) f) --> l) sequentially``,
+ ``!f l k. (f sums l) (from k) = ((\n. sum{k..n} f) --> l) sequentially``,
   REPEAT GEN_TAC THEN REWRITE_TAC[sums] THEN
   AP_THM_TAC THEN AP_THM_TAC THEN AP_TERM_TAC THEN ABS_TAC THEN
   AP_THM_TAC THEN AP_TERM_TAC THEN
@@ -17467,7 +17467,7 @@ val SERIES_FINITE = store_thm ("SERIES_FINITE",
   X_GEN_TAC ``n:num`` THEN SIMP_TAC std_ss [sums, LIM_SEQUENTIALLY] THEN
   DISCH_TAC THEN X_GEN_TAC ``e:real`` THEN DISCH_TAC THEN EXISTS_TAC ``n:num`` THEN
   X_GEN_TAC ``m:num`` THEN DISCH_TAC THEN
-  SUBGOAL_THEN ``s INTER ((0:num)..m) = s``
+  SUBGOAL_THEN ``s INTER { 0n..m} = s``
    (fn th => ASM_REWRITE_TAC[th, DIST_REFL]) THEN
   SIMP_TAC std_ss [EXTENSION, IN_INTER, IN_NUMSEG, ZERO_LESS_EQ] THEN
   METIS_TAC[LESS_EQ_TRANS]);
@@ -17524,7 +17524,7 @@ val SERIES_FINITE_SUPPORT = store_thm ("SERIES_FINITE_SUPPORT",
   EXISTS_TAC ``N:num`` THEN POP_ASSUM MP_TAC THEN
   STRIP_TAC THEN X_GEN_TAC ``n:num`` THEN DISCH_TAC THEN
   SIMP_TAC std_ss [] THEN
-  SUBGOAL_THEN ``sum (k INTER ((0:num)..n)) (f:num->real) = sum(s INTER k) f``
+  SUBGOAL_THEN ``sum (k INTER { 0n..n}) (f:num->real) = sum(s INTER k) f``
    (fn th => ASM_SIMP_TAC std_ss [DIST_REFL, th]) THEN
   MATCH_MP_TAC SUM_SUPERSET THEN
   ASM_SIMP_TAC std_ss [SUBSET_DEF, IN_INTER, IN_NUMSEG, ZERO_LESS_EQ] THEN
@@ -17710,9 +17710,9 @@ val SUMS_FINITE_UNION = store_thm ("SUMS_FINITE_UNION",
 val SUMS_OFFSET = store_thm ("SUMS_OFFSET",
  ``!f l:real m n.
            (f sums l) (from m) /\ 0 < n /\ m <= n
-           ==> (f sums l - sum (m..n - 1) f) (from n)``,
+           ==> (f sums l - sum {m..n - 1} f) (from n)``,
   REPEAT STRIP_TAC THEN
-  SUBGOAL_THEN ``from n = from m DIFF (m..(n-1:num))`` SUBST1_TAC THENL
+  SUBGOAL_THEN ``from n = from m DIFF {m..n-1}`` SUBST1_TAC THENL
    [SIMP_TAC std_ss [EXTENSION, IN_FROM, IN_DIFF, IN_NUMSEG] THEN
     GEN_TAC THEN EQ_TAC THENL [DISCH_TAC THEN CONJ_TAC THENL
      [MATCH_MP_TAC LESS_EQ_TRANS THEN EXISTS_TAC ``n:num`` THEN ASM_REWRITE_TAC [],
@@ -17726,9 +17726,9 @@ val SUMS_OFFSET = store_thm ("SUMS_OFFSET",
 val SUMS_OFFSET_REV = store_thm ("SUMS_OFFSET_REV",
  ``!f:num->real l m n.
         (f sums l) (from m) /\ 0 < m /\ n <= m
-        ==> (f sums (l + sum(n..m-1) f)) (from n)``,
+        ==> (f sums (l + sum{n..m-1} f)) (from n)``,
   REPEAT STRIP_TAC THEN
-  MP_TAC(ISPECL [``f:num->real``, ``from m``, ``n..m-1``, ``l:real``]
+  MP_TAC(ISPECL [``f:num->real``, ``from m``, ``{n..m-1}``, ``l:real``]
                 SUMS_FINITE_UNION) THEN
   ASM_REWRITE_TAC[FINITE_NUMSEG] THEN MATCH_MP_TAC EQ_IMPLIES THEN
   BINOP_TAC THENL [AP_TERM_TAC THEN AP_THM_TAC THEN AP_TERM_TAC, ALL_TAC] THEN
@@ -17747,8 +17747,8 @@ val SERIES_DROP_LE = store_thm ("SERIES_DROP_LE",
   REWRITE_TAC[sums] THEN REPEAT STRIP_TAC THEN
   MATCH_MP_TAC(ISPEC ``sequentially`` LIM_DROP_LE) THEN
   REWRITE_TAC[EVENTUALLY_SEQUENTIALLY, TRIVIAL_LIMIT_SEQUENTIALLY] THEN
-  EXISTS_TAC ``\n. sum (s INTER ((0:num)..n)) (f:num->real)`` THEN
-  EXISTS_TAC ``\n. sum (s INTER ((0:num)..n)) (g:num->real)`` THEN
+  EXISTS_TAC ``\n. sum (s INTER { 0n..n}) (f:num->real)`` THEN
+  EXISTS_TAC ``\n. sum (s INTER { 0n..n}) (g:num->real)`` THEN
   ASM_REWRITE_TAC[] THEN EXISTS_TAC ``0:num`` THEN REPEAT STRIP_TAC THEN
   SIMP_TAC std_ss [] THEN MATCH_MP_TAC SUM_LE THEN
   ASM_SIMP_TAC std_ss [FINITE_INTER, FINITE_NUMSEG, IN_INTER, IN_NUMSEG]);
@@ -17769,12 +17769,12 @@ val SERIES_BOUND = store_thm ("SERIES_BOUND",
         ==> abs (a) <= b``,
   REWRITE_TAC[sums] THEN REPEAT STRIP_TAC THEN
   MATCH_MP_TAC(ISPEC ``sequentially`` LIM_ABS_UBOUND) THEN
-  EXISTS_TAC ``\n. sum (s INTER ((0:num)..n)) (f:num->real)`` THEN
+  EXISTS_TAC ``\n. sum (s INTER { 0n..n}) (f:num->real)`` THEN
   ASM_REWRITE_TAC[TRIVIAL_LIMIT_SEQUENTIALLY] THEN
   REWRITE_TAC[EVENTUALLY_SEQUENTIALLY] THEN EXISTS_TAC ``0:num`` THEN
   X_GEN_TAC ``m:num`` THEN DISCH_TAC THEN
   SIMP_TAC std_ss [] THEN MATCH_MP_TAC REAL_LE_TRANS THEN
-  EXISTS_TAC ``sum (s INTER ((0:num)..m)) g`` THEN CONJ_TAC THEN
+  EXISTS_TAC ``sum (s INTER { 0n..m}) g`` THEN CONJ_TAC THEN
   ASM_SIMP_TAC std_ss [SUM_ABS_LE, IN_INTER, FINITE_NUMSEG, FINITE_INTER] THEN
   RULE_ASSUM_TAC(REWRITE_RULE[GSYM sums]) THEN
   UNDISCH_TAC ``(g sums b) s`` THEN
@@ -17850,26 +17850,26 @@ val INFSUM_RESTRICT = store_thm ("INFSUM_RESTRICT",
 val PARTIAL_SUMS_COMPONENT_LE_INFSUM = store_thm ("PARTIAL_SUMS_COMPONENT_LE_INFSUM",
  ``!f:num->real s n.
         (!i. i IN s ==> &0 <= f i) /\ summable s f
-        ==> (sum (s INTER ((0:num)..n)) f) <= (infsum s f)``,
+        ==> (sum (s INTER { 0n..n}) f) <= (infsum s f)``,
   REPEAT GEN_TAC THEN REWRITE_TAC[GSYM SUMS_INFSUM] THEN
   REPEAT(DISCH_THEN(CONJUNCTS_THEN2 ASSUME_TAC MP_TAC)) THEN
   REWRITE_TAC[sums, LIM_SEQUENTIALLY] THEN DISCH_TAC THEN
   REWRITE_TAC[GSYM REAL_NOT_LT] THEN DISCH_TAC THEN
   FIRST_X_ASSUM(MP_TAC o SPEC
-   ``sum (s INTER ((0:num)..n)) (f:num->real) - (infsum s f)``) THEN
+   ``sum (s INTER { 0n..n}) (f:num->real) - (infsum s f)``) THEN
   ASM_REWRITE_TAC[REAL_SUB_LT] THEN
   DISCH_THEN(X_CHOOSE_THEN ``N:num`` (MP_TAC o SPEC ``N + n:num``)) THEN
   REWRITE_TAC[LE_ADD, REAL_NOT_LT, dist] THEN
   MATCH_MP_TAC REAL_LE_TRANS THEN
-  EXISTS_TAC ``abs((sum (s INTER ((0:num)..N + n)) f - infsum s f:real))`` THEN
+  EXISTS_TAC ``abs((sum (s INTER { 0n..N + n}) f - infsum s f:real))`` THEN
   ASM_SIMP_TAC std_ss [REAL_LE_REFL] THEN
   MATCH_MP_TAC(REAL_ARITH ``s < a /\ a <= b ==> a - s <= abs(b - s:real)``) THEN
   ASM_REWRITE_TAC[] THEN ONCE_REWRITE_TAC[ADD_SYM] THEN
-  KNOW_TAC ``sum (s INTER ((0:num)..n)) f <=
-              sum (s INTER ((0:num)..n) UNION s INTER (n + (1:num)..n + N)) f`` THENL
+  KNOW_TAC ``sum (s INTER { 0n..n}) f <=
+              sum (s INTER { 0n..n} UNION s INTER {n +  1n..n + N}) f`` THENL
   [ALL_TAC, SIMP_TAC std_ss [GSYM NUMSEG_ADD_SPLIT, ZERO_LESS_EQ, GSYM UNION_OVER_INTER]] THEN
-  KNOW_TAC ``(sum (s INTER ((0:num)..n) UNION s INTER (n + (1:num)..n + N)) f =
-              sum (s INTER ((0:num)..n)) f + sum (s INTER (n + (1:num)..n + N)) f)`` THENL
+  KNOW_TAC ``(sum (s INTER { 0n..n} UNION s INTER {n +  1n..n + N}) f =
+              sum (s INTER { 0n..n}) f + sum (s INTER {n +  1n..n + N}) f)`` THENL
   [MATCH_MP_TAC SUM_UNION THEN
    SIMP_TAC std_ss [FINITE_INTER, FINITE_NUMSEG, DISJOINT_DEF, EXTENSION] THEN
    SIMP_TAC arith_ss [IN_INTER, NOT_IN_EMPTY, IN_NUMSEG] THEN CCONTR_TAC THEN
@@ -17883,7 +17883,7 @@ val PARTIAL_SUMS_DROP_LE_INFSUM = store_thm ("PARTIAL_SUMS_DROP_LE_INFSUM",
  ``!f s n.
         (!i. i IN s ==> &0 <= f i) /\
         summable s f
-        ==> sum (s INTER ((0:num)..n)) f <= (infsum s f)``,
+        ==> sum (s INTER { 0n..n}) f <= (infsum s f)``,
   REPEAT STRIP_TAC THEN
   MATCH_MP_TAC PARTIAL_SUMS_COMPONENT_LE_INFSUM THEN
   ASM_REWRITE_TAC[LESS_EQ_REFL]);
@@ -17900,13 +17900,13 @@ val SEQUENCE_CAUCHY_WLOG = store_thm ("SEQUENCE_CAUCHY_WLOG",
 val SUM_DIFF_LEMMA = store_thm ("SUM_DIFF_LEMMA",
  ``!f:num->real k m n.
         m <= n
-        ==> (sum (k INTER ((0:num) .. n)) f - sum (k INTER ((0:num)..m)) f =
-             sum (k INTER ((m+1:num) .. n)) f)``,
+        ==> (sum (k INTER {0 .. n}) f - sum (k INTER { 0n..m}) f =
+             sum (k INTER {m+1 .. n}) f)``,
   REPEAT STRIP_TAC THEN
-  MP_TAC(ISPECL [``f:num->real``, ``k INTER ((0:num)..n)``, ``k INTER ((0:num)..m)``]
+  MP_TAC(ISPECL [``f:num->real``, ``k INTER { 0n..n}``, ``k INTER { 0n..m}``]
     SUM_DIFF) THEN
-  KNOW_TAC ``FINITE (k INTER ((0:num) .. n)) /\
-             k INTER ((0:num) .. m) SUBSET k INTER ((0:num) .. n)`` THENL
+  KNOW_TAC ``FINITE (k INTER { 0n .. n}) /\
+             k INTER { 0n .. m} SUBSET k INTER { 0n .. n}`` THENL
    [SIMP_TAC std_ss [FINITE_INTER, FINITE_NUMSEG] THEN MATCH_MP_TAC
      (SET_RULE ``s SUBSET t ==> (u INTER s SUBSET u INTER t)``) THEN
     REWRITE_TAC[SUBSET_DEF, IN_NUMSEG] THEN POP_ASSUM MP_TAC THEN ARITH_TAC,
@@ -17918,8 +17918,8 @@ val SUM_DIFF_LEMMA = store_thm ("SUM_DIFF_LEMMA",
     POP_ASSUM MP_TAC THEN ARITH_TAC]);
 
 val ABS_SUM_TRIVIAL_LEMMA = store_thm ("ABS_SUM_TRIVIAL_LEMMA",
- ``!e:real. &0 < e ==> (P ==> abs(sum(s INTER (m..n)) f) < e <=>
-                        P ==> n < m \/ abs(sum(s INTER (m..n)) f) < e)``,
+ ``!e:real. &0 < e ==> (P ==> abs(sum(s INTER {m..n}) f) < e <=>
+                        P ==> n < m \/ abs(sum(s INTER {m..n}) f) < e)``,
   REPEAT STRIP_TAC THEN ASM_CASES_TAC ``n:num < m`` THEN ASM_REWRITE_TAC[] THEN
   FIRST_X_ASSUM(SUBST1_TAC o REWRITE_RULE [GSYM NUMSEG_EMPTY]) THEN
   ASM_REWRITE_TAC[SUM_CLAUSES, ABS_0, INTER_EMPTY]);
@@ -17928,7 +17928,7 @@ val SERIES_CAUCHY = store_thm ("SERIES_CAUCHY",
  ``!f s. (?l. (f sums l) s) =
          !e. &0 < e
              ==> ?N. !m n. m >= N
-                           ==> abs(sum(s INTER (m..n)) f) < e``,
+                           ==> abs(sum(s INTER {m..n}) f) < e``,
   REPEAT GEN_TAC THEN REWRITE_TAC[sums, CONVERGENT_EQ_CAUCHY, cauchy] THEN
   SIMP_TAC std_ss [SEQUENCE_CAUCHY_WLOG] THEN ONCE_REWRITE_TAC[DIST_SYM] THEN
   SIMP_TAC std_ss [dist, SUM_DIFF_LEMMA, ABS_SUM_TRIVIAL_LEMMA] THEN
@@ -17952,7 +17952,7 @@ val SERIES_CAUCHY = store_thm ("SERIES_CAUCHY",
 val SUMMABLE_CAUCHY = store_thm ("SUMMABLE_CAUCHY",
  ``!f s. summable s f <=>
          !e. &0 < e
-             ==> ?N. !m n. m >= N ==> abs(sum(s INTER (m..n)) f) < e``,
+             ==> ?N. !m n. m >= N ==> abs(sum(s INTER {m..n}) f) < e``,
   REWRITE_TAC[summable, GSYM SERIES_CAUCHY]);
 
 val SUMMABLE_IFF_EVENTUALLY = store_thm ("SUMMABLE_IFF_EVENTUALLY",
@@ -17999,7 +17999,7 @@ val SUMMABLE_FROM_ELSEWHERE = store_thm ("SUMMABLE_FROM_ELSEWHERE",
  ``!f m n. summable (from m) f ==> summable (from n) f``,
   REPEAT GEN_TAC THEN
   MATCH_MP_TAC(REWRITE_RULE[CONJ_EQ_IMP] SUMMABLE_EQ_COFINITE) THEN
-  MATCH_MP_TAC SUBSET_FINITE_I THEN EXISTS_TAC ``(0:num)..(m+n)`` THEN
+  MATCH_MP_TAC SUBSET_FINITE_I THEN EXISTS_TAC ``{0n..m+n}`` THEN
   SIMP_TAC std_ss [FINITE_NUMSEG, SUBSET_DEF, IN_NUMSEG, IN_UNION, IN_DIFF, IN_FROM] THEN
   ARITH_TAC);
 
@@ -18011,16 +18011,16 @@ val SERIES_CAUCHY_UNIFORM = store_thm ("SERIES_CAUCHY_UNIFORM",
  ``!P f:'a->num->real k.
         (?l. !e. &0 < e
                  ==> ?N. !n x. N <= n /\ P x
-                               ==> dist(sum(k INTER ((0:num)..n)) (f x),
+                               ==> dist(sum(k INTER { 0n..n}) (f x),
                                         l x) < e) <=>
         (!e. &0 < e ==> ?N. !m n x. N <= m /\ P x
-                                    ==> abs(sum(k INTER (m..n)) (f x)) < e)``,
+                                    ==> abs(sum(k INTER {m..n}) (f x)) < e)``,
   REPEAT GEN_TAC THEN
   SIMP_TAC std_ss [sums, UNIFORMLY_CONVERGENT_EQ_CAUCHY, cauchy] THEN
-  ONCE_REWRITE_TAC [METIS [] ``(dist (sum (k INTER (0 .. n)) (f x),
-                                      sum (k INTER (0 .. n')) (f x)) < e) =
-                      (\n n' x. dist (sum (k INTER (0 .. n)) (f x),
-                                      sum (k INTER (0 .. n')) (f x)) < e) n n' x``] THEN
+  ONCE_REWRITE_TAC [METIS [] ``(dist (sum (k INTER {0 .. n}) (f x),
+                                      sum (k INTER {0 .. n'}) (f x)) < e) =
+                      (\n n' x. dist (sum (k INTER {0 .. n}) (f x),
+                                      sum (k INTER {0 .. n'}) (f x)) < e) n n' x``] THEN
   ONCE_REWRITE_TAC[MESON[]
    ``(!m n:num y. N <= m /\ N <= n /\ P y ==> Q m n y) <=>
      (!y. P y ==> !m n. N <= m /\ N <= n ==> Q m n y)``] THEN
@@ -18072,7 +18072,7 @@ val SUMMABLE_IMP_TOZERO = store_thm ("SUMMABLE_IMP_TOZERO",
   X_GEN_TAC ``N:num`` THEN DISCH_TAC THEN EXISTS_TAC ``N + 1:num`` THEN
   X_GEN_TAC ``n:num`` THEN DISCH_TAC THEN
   UNDISCH_TAC ``!n:num. N <= n ==>
-        dist (sum ((0:num) .. n) (\n. if n IN k then f n else 0),l) < e / 2:real`` THEN
+        dist (sum { 0n .. n} (\n. if n IN k then f n else 0),l) < e / 2:real`` THEN
   DISCH_TAC THEN
   FIRST_X_ASSUM(fn th =>
     MP_TAC(SPEC ``n - 1:num`` th) THEN MP_TAC(SPEC ``n:num`` th)) THEN
@@ -18096,7 +18096,7 @@ val SUMMABLE_IMP_BOUNDED = store_thm ("SUMMABLE_IMP_BOUNDED",
 
 val SUMMABLE_IMP_SUMS_BOUNDED = store_thm ("SUMMABLE_IMP_SUMS_BOUNDED",
  ``!f:num->real k.
-       summable (from k) f ==> bounded { sum(k..n) f | n IN univ(:num) }``,
+       summable (from k) f ==> bounded { sum{k..n} f | n IN univ(:num) }``,
   SIMP_TAC std_ss [summable, sums, LEFT_IMP_EXISTS_THM] THEN REPEAT GEN_TAC THEN
   DISCH_THEN(MP_TAC o MATCH_MP CONVERGENT_IMP_BOUNDED) THEN
   SIMP_TAC std_ss [FROM_INTER_NUMSEG, GSYM IMAGE_DEF]);
@@ -18117,7 +18117,7 @@ val SERIES_COMPARISON = store_thm ("SERIES_COMPARISON",
   EXISTS_TAC ``N1 + N2:num`` THEN
   MAP_EVERY X_GEN_TAC [``m:num``, ``n:num``] THEN DISCH_TAC THEN
   MATCH_MP_TAC REAL_LET_TRANS THEN
-  EXISTS_TAC ``abs (sum (s INTER (m .. n)) g)`` THEN CONJ_TAC THENL
+  EXISTS_TAC ``abs (sum (s INTER {m .. n}) g)`` THEN CONJ_TAC THENL
    [SIMP_TAC std_ss [FINITE_INTER_NUMSEG] THEN
     MATCH_MP_TAC(REAL_ARITH ``x <= a ==> x <= abs(a:real)``) THEN
     MATCH_MP_TAC SUM_ABS_LE THEN
@@ -18177,7 +18177,7 @@ val SERIES_COMPARISON_UNIFORM = store_thm ("SERIES_COMPARISON_UNIFORM",
              ==> ?l:'a->real.
                     !e. &0 < e
                         ==> ?N. !n x. N <= n /\ P x
-                                      ==> dist(sum(s INTER ((0:num)..n)) (f x),
+                                      ==> dist(sum(s INTER { 0n..n}) (f x),
                                                l x) < e``,
   REPEAT GEN_TAC THEN SIMP_TAC std_ss [GE, SERIES_CAUCHY, SERIES_CAUCHY_UNIFORM] THEN
   DISCH_THEN(CONJUNCTS_THEN2 MP_TAC (X_CHOOSE_TAC ``N1:num``)) THEN
@@ -18187,7 +18187,7 @@ val SERIES_COMPARISON_UNIFORM = store_thm ("SERIES_COMPARISON_UNIFORM",
   EXISTS_TAC ``N1 + N2:num`` THEN
   MAP_EVERY X_GEN_TAC [``m:num``, ``n:num``, ``x:'a``] THEN DISCH_TAC THEN
   MATCH_MP_TAC REAL_LET_TRANS THEN
-  EXISTS_TAC ``abs (sum (s INTER (m .. n)) g)`` THEN CONJ_TAC THENL
+  EXISTS_TAC ``abs (sum (s INTER {m .. n}) g)`` THEN CONJ_TAC THENL
    [SIMP_TAC std_ss [FINITE_INTER_NUMSEG] THEN
     MATCH_MP_TAC(REAL_ARITH ``x <= a ==> x <= abs(a:real)``) THEN
     MATCH_MP_TAC SUM_ABS_LE THEN
@@ -18242,7 +18242,7 @@ val SERIES_RATIO = store_thm ("SERIES_RATIO",
   MAP_EVERY X_GEN_TAC [``m:num``, ``n:num``] THEN DISCH_TAC THEN
   MATCH_MP_TAC REAL_LET_TRANS THEN
   EXISTS_TAC ``abs(abs((a:num->real) N) *
-                  sum(m..n) (\i. c pow (i - N)))`` THEN
+                  sum{m..n} (\i. c pow (i - N)))`` THEN
   CONJ_TAC THENL
    [REWRITE_TAC[ABS_MUL] THEN MATCH_MP_TAC REAL_LE_LMUL_IMP THEN
     REWRITE_TAC[ABS_POS] THEN
@@ -18299,10 +18299,10 @@ val SERIES_RATIO = store_thm ("SERIES_RATIO",
 
 val BOUNDED_PARTIAL_SUMS = store_thm ("BOUNDED_PARTIAL_SUMS",
  ``!f:num->real k.
-        bounded { sum(k..n) f | n IN univ(:num) }
-        ==> bounded { sum(m..n) f | m IN univ(:num) /\ n IN univ(:num) }``,
+        bounded { sum{k..n} f | n IN univ(:num) }
+        ==> bounded { sum{m..n} f | m IN univ(:num) /\ n IN univ(:num) }``,
   REPEAT STRIP_TAC THEN
-  SUBGOAL_THEN ``bounded { sum((0:num)..n) f:real | n IN univ(:num) }`` MP_TAC THENL
+  SUBGOAL_THEN ``bounded { sum{ 0n..n} f:real | n IN univ(:num) }`` MP_TAC THENL
    [FIRST_X_ASSUM(MP_TAC o REWRITE_RULE [BOUNDED_POS]) THEN
     REWRITE_TAC[bounded_def] THEN
     SIMP_TAC real_ss [GSYM IMAGE_DEF, FORALL_IN_IMAGE, IN_UNIV] THEN
@@ -18311,7 +18311,7 @@ val BOUNDED_PARTIAL_SUMS = store_thm ("BOUNDED_PARTIAL_SUMS",
     X_GEN_TAC ``i:num`` THEN ASM_CASES_TAC ``i:num < k`` THENL
      [MATCH_MP_TAC(REAL_ARITH
        ``!y. x <= y /\ y <= a /\ &0 < b ==> x <= a + b:real``) THEN
-      EXISTS_TAC ``sum ((0:num)..i) (\i. abs(f i:real))`` THEN
+      EXISTS_TAC ``sum { 0n..i} (\i. abs(f i:real))`` THEN
       ASM_SIMP_TAC std_ss [SUM_ABS, FINITE_NUMSEG] THEN
       MATCH_MP_TAC SUM_SUBSET THEN
       REWRITE_TAC[FINITE_NUMSEG, FINITE_NUMSEG_LT, ABS_POS] THEN
@@ -18339,10 +18339,10 @@ val BOUNDED_PARTIAL_SUMS = store_thm ("BOUNDED_PARTIAL_SUMS",
   MATCH_MP_TAC(REWRITE_RULE[TAUT `a /\ b ==> c <=> b ==> a ==> c`]
         BOUNDED_SUBSET) THEN
   KNOW_TAC ``!x:real m n:num.
-     (x = sum (m..n) f)
-     ==> (?n. x = sum ((0:num)..n) f) \/
+     (x = sum {m..n} f)
+     ==> (?n. x = sum { 0n..n} f) \/
          (?x' y.
-              ((?n. x' = sum ((0:num)..n) f) /\ (?n. y = sum ((0:num)..n) f)) /\
+              ((?n. x' = sum { 0n..n} f) /\ (?n. y = sum { 0n..n} f)) /\
               (x = x' - y))`` THENL
   [ALL_TAC, SIMP_TAC std_ss [SUBSET_DEF, GSPECIFICATION, IN_UNION, LEFT_IMP_EXISTS_THM,
                              IN_UNIV, EXISTS_PROD] THEN METIS_TAC []] THEN
@@ -18350,11 +18350,11 @@ val BOUNDED_PARTIAL_SUMS = store_thm ("BOUNDED_PARTIAL_SUMS",
   DISCH_THEN SUBST1_TAC THEN
   ASM_CASES_TAC ``m = 0:num`` THENL [ASM_MESON_TAC[], ALL_TAC] THEN
   ASM_CASES_TAC ``n:num < m`` THENL
-   [DISJ2_TAC THEN REPEAT(EXISTS_TAC ``sum((0:num)..(0:num)) (f:num->real)``) THEN
+   [DISJ2_TAC THEN REPEAT(EXISTS_TAC ``sum{ 0n.. 0n} (f:num->real)``) THEN
     ASM_SIMP_TAC std_ss [SUM_TRIV_NUMSEG, REAL_SUB_REFL] THEN MESON_TAC[],
     ALL_TAC] THEN
   DISJ2_TAC THEN MAP_EVERY EXISTS_TAC
-   [``sum((0:num)..n) (f:num->real)``, ``sum((0:num)..(m-1:num)) (f:num->real)``] THEN
+   [``sum{0..n} (f:num->real)``, ``sum{0..m-1} (f:num->real)``] THEN
   CONJ_TAC THENL [MESON_TAC[], ALL_TAC] THEN
   MP_TAC(ISPECL [``f:num->real``, ``0:num``, ``m:num``, ``n:num``]
       SUM_COMBINE_L) THEN ASM_SIMP_TAC arith_ss [] THEN
@@ -18379,26 +18379,26 @@ val SUMMABLE_BILINEAR_PARTIAL_PRE = store_thm ("SUMMABLE_BILINEAR_PARTIAL_PRE",
   EXISTS_TAC ``l - (h:real->real->real) ((f:num->real) k) (g(k - 1)) - l'`` THEN
   SIMP_TAC std_ss [LIM_CASES_SEQUENTIALLY] THEN
   KNOW_TAC  ``(((\(n :num).
-     (\n. (h :real -> real -> real) ((f :num -> real) (n + (1 :num)))
-       ((g :num -> real) n) - h (f (k :num)) (g (k - (1 :num)))) n -
-     (\n. sum (k .. n) (\(k :num). h (f (k + (1 :num)) - f k) (g k))) n) -->
-  ((l :real) - h (f k) (g (k - (1 :num))) - (l' :real))) sequentially :
+     (\n. (h :real -> real -> real) ((f :num -> real) (n +  1n))
+       ((g :num -> real) n) - h (f (k :num)) (g (k -  1n))) n -
+     (\n. sum {k .. n} (\(k :num). h (f (k +  1n) - f k) (g k))) n) -->
+  ((l :real) - h (f k) (g (k -  1n)) - (l' :real))) sequentially :
    bool)`` THENL
   [ALL_TAC, METIS_TAC []] THEN
   MATCH_MP_TAC LIM_SUB THEN ASM_SIMP_TAC std_ss [LIM_CONST] THEN
   KNOW_TAC ``(((\(n :num).
-     (\n. (h :real -> real -> real) ((f :num -> real) (n + (1 :num)))
-       ((g :num -> real) n)) n - (\n. h (f (k :num)) (g (k - (1 :num)))) n) -->
-  ((l :real) - h (f k) (g (k - (1 :num))))) sequentially :bool)`` THENL
+     (\n. (h :real -> real -> real) ((f :num -> real) (n +  1n))
+       ((g :num -> real) n)) n - (\n. h (f (k :num)) (g (k -  1n))) n) -->
+  ((l :real) - h (f k) (g (k -  1n)))) sequentially :bool)`` THENL
   [ALL_TAC, METIS_TAC []] THEN MATCH_MP_TAC LIM_SUB THEN
   ASM_SIMP_TAC std_ss [LIM_CONST]);
 
 val SERIES_DIRICHLET_BILINEAR = store_thm ("SERIES_DIRICHLET_BILINEAR",
  ``!f g h:real->real->real k m p l.
         bilinear h /\
-        bounded {sum (m..n) f | n IN univ(:num)} /\
+        bounded {sum {m..n} f | n IN univ(:num)} /\
         summable (from p) (\n. abs(g(n + 1) - g(n))) /\
-        ((\n. h (g(n + 1)) (sum((1:num)..n) f)) --> l) sequentially
+        ((\n. h (g(n + 1)) (sum{ 1n..n} f)) --> l) sequentially
         ==> summable (from k) (\n. h (g n) (f n))``,
   REPEAT STRIP_TAC THEN MATCH_MP_TAC SUMMABLE_FROM_ELSEWHERE THEN
   EXISTS_TAC ``1:num`` THEN
@@ -18410,7 +18410,7 @@ val SERIES_DIRICHLET_BILINEAR = store_thm ("SERIES_DIRICHLET_BILINEAR",
   DISCH_THEN(X_CHOOSE_THEN ``C:real`` STRIP_ASSUME_TAC) THEN
   MATCH_MP_TAC SUMMABLE_EQ THEN
   EXISTS_TAC ``\n. (h:real->real->real)
-                   (g n) (sum ((1:num)..n) f - sum ((1:num)..n-1:num) f)`` THEN
+                   (g n) (sum { 1n..n} f - sum { 1n..n-1:num} f)`` THEN
   SIMP_TAC std_ss [IN_FROM, GSYM NUMSEG_RREC] THEN
   SIMP_TAC std_ss [SUM_CLAUSES, FINITE_NUMSEG, IN_NUMSEG,
            ARITH_PROVE ``1 <= n ==> ~(n <= n - 1:num)``] THEN
@@ -18419,7 +18419,7 @@ val SERIES_DIRICHLET_BILINEAR = store_thm ("SERIES_DIRICHLET_BILINEAR",
     REAL_ARITH_TAC,
     ALL_TAC] THEN
   MATCH_MP_TAC SUMMABLE_FROM_ELSEWHERE THEN EXISTS_TAC ``p:num`` THEN
-  MP_TAC(ISPECL [``g:num->real``, ``\n. sum((1:num)..n) f:real``,
+  MP_TAC(ISPECL [``g:num->real``, ``\n. sum{ 1n..n} f:real``,
                  ``h:real->real->real``, ``l:real``, ``p:num``]
          SUMMABLE_BILINEAR_PARTIAL_PRE) THEN
   SIMP_TAC std_ss [] THEN DISCH_THEN MATCH_MP_TAC THEN
@@ -18430,7 +18430,7 @@ val SERIES_DIRICHLET_BILINEAR = store_thm ("SERIES_DIRICHLET_BILINEAR",
   MATCH_MP_TAC(REWRITE_RULE[IMP_CONJ_ALT] SUMMABLE_COMPARISON) THEN
   EXISTS_TAC ``0:num`` THEN REWRITE_TAC[IN_FROM, GE, ZERO_LESS_EQ] THEN
   REPEAT STRIP_TAC THEN MATCH_MP_TAC REAL_LE_TRANS THEN EXISTS_TAC
-   ``C * abs(g(n + 1:num) - g(n):real) * abs(sum ((1:num)..n) f:real)`` THEN
+   ``C * abs(g(n + 1:num) - g(n):real) * abs(sum { 1n..n} f:real)`` THEN
   ASM_SIMP_TAC std_ss [REAL_LE_LMUL] THEN
   REWRITE_TAC [GSYM REAL_MUL_ASSOC] THEN
   ASM_SIMP_TAC std_ss [REAL_LE_LMUL] THEN
@@ -18439,7 +18439,7 @@ val SERIES_DIRICHLET_BILINEAR = store_thm ("SERIES_DIRICHLET_BILINEAR",
 
 val SERIES_DIRICHLET = store_thm ("SERIES_DIRICHLET",
  ``!f:num->real g N k m.
-        bounded {sum (m..n) f | n IN univ(:num)} /\
+        bounded {sum {m..n} f | n IN univ(:num)} /\
         (!n. N <= n ==> g(n + 1) <= g(n)) /\
         (g --> 0) sequentially
         ==> summable (from k) (\n. g(n) * f(n))``,
@@ -18469,8 +18469,8 @@ val SERIES_DIRICHLET = store_thm ("SERIES_DIRICHLET",
       MATCH_MP_TAC LIM_SUB THEN ASM_REWRITE_TAC[LIM_CONST]],
     ONCE_REWRITE_TAC [REAL_MUL_SYM] THEN
     ONCE_REWRITE_TAC [METIS []
-        ``((\n. sum (1 .. n) f * (g:num->real) (n + 1)) --> 0) =
-      ((\n. (\n. sum (1 .. n) f) n * (\n. g (n + 1)) n) --> 0)``] THEN
+        ``((\n. sum {1 .. n} f * (g:num->real) (n + 1)) --> 0) =
+      ((\n. (\n. sum {1 .. n} f) n * (\n. g (n + 1)) n) --> 0)``] THEN
     MATCH_MP_TAC LIM_NULL_CMUL_BOUNDED THEN ASM_SIMP_TAC std_ss [o_DEF] THEN
     REWRITE_TAC[EVENTUALLY_SEQUENTIALLY] THEN
     FIRST_X_ASSUM(ASSUME_TAC o MATCH_MP BOUNDED_PARTIAL_SUMS) THEN
@@ -18495,8 +18495,8 @@ val SERIES_INJECTIVE_IMAGE_STRONG = store_thm ("SERIES_INJECTIVE_IMAGE_STRONG",
  ``!x:num->real s f.
         summable (IMAGE f s) (\n. abs(x n)) /\
         (!m n. m IN s /\ n IN s /\ (f m = f n) ==> (m = n))
-        ==> ((\n. sum (IMAGE f s INTER ((0:num)..n)) x -
-                  sum (s INTER ((0:num)..n)) (x o f)) --> 0)
+        ==> ((\n. sum (IMAGE f s INTER { 0n..n}) x -
+                  sum (s INTER { 0n..n}) (x o f)) --> 0)
             sequentially``,
   REPEAT STRIP_TAC THEN REWRITE_TAC[LIM_SEQUENTIALLY] THEN
   X_GEN_TAC ``e:real`` THEN DISCH_TAC THEN
@@ -18514,7 +18514,7 @@ val SERIES_INJECTIVE_IMAGE_STRONG = store_thm ("SERIES_INJECTIVE_IMAGE_STRONG",
         (m = n)`` THEN DISCH_TAC THEN
   FIRST_ASSUM(MP_TAC o REWRITE_RULE [INJECTIVE_ON_LEFT_INVERSE]) THEN
   DISCH_THEN(X_CHOOSE_TAC ``g:num->num``) THEN
-  MP_TAC(ISPECL [``g:num->num``, ``((0:num)..N)``] UPPER_BOUND_FINITE_SET) THEN
+  MP_TAC(ISPECL [``g:num->num``, ``{ 0n..N}``] UPPER_BOUND_FINITE_SET) THEN
   REWRITE_TAC[FINITE_NUMSEG, IN_NUMSEG, ZERO_LESS_EQ] THEN
   DISCH_THEN(X_CHOOSE_TAC ``P:num``) THEN
   EXISTS_TAC ``MAX N P:num`` THEN X_GEN_TAC ``n:num`` THEN
@@ -18524,8 +18524,8 @@ val SERIES_INJECTIVE_IMAGE_STRONG = store_thm ("SERIES_INJECTIVE_IMAGE_STRONG",
   W(MP_TAC o PART_MATCH (rand o rand) SUM_IMAGE o rand o
     rand o lhand o snd) THEN
   KNOW_TAC ``(!(x :num) (y :num).
-    x IN (s :num -> bool) INTER ((0 :num) .. (n :num)) /\
-    y IN s INTER ((0 :num) .. n) /\ ((f :num -> num) x = f y) ==>
+    x IN (s :num -> bool) INTER {0 .. n} /\
+    y IN s INTER { 0 .. n} /\ ((f :num -> num) x = f y) ==>
     (x = y))`` THENL
    [ASM_MESON_TAC[FINITE_INTER, FINITE_NUMSEG, IN_INTER],
     DISCH_TAC THEN ASM_REWRITE_TAC [] THEN POP_ASSUM K_TAC THEN
@@ -18541,7 +18541,7 @@ val SERIES_INJECTIVE_IMAGE_STRONG = store_thm ("SERIES_INJECTIVE_IMAGE_STRONG",
   MATCH_MP_TAC(REWRITE_RULE[IMP_CONJ_ALT] REAL_LET_TRANS) THEN
   MATCH_MP_TAC REAL_LET_TRANS THENL
    [EXISTS_TAC
-     ``sum((IMAGE (f:num->num) s) INTER (N..n)) (\i. abs(x i :real))`` THEN
+     ``sum((IMAGE (f:num->num) s) INTER {N..n}) (\i. abs(x i :real))`` THEN
     CONJ_TAC THENL [ALL_TAC,
      MATCH_MP_TAC (REAL_ARITH ``abs x < y ==> x < y:real``) THEN
      ASM_SIMP_TAC real_ss []] THEN
@@ -18557,11 +18557,11 @@ val SERIES_INJECTIVE_IMAGE_STRONG = store_thm ("SERIES_INJECTIVE_IMAGE_STRONG",
     UNDISCH_TAC ``!(x :num). x <= (N :num) ==> (g :num -> num) x <= (P :num)`` THEN
     DISCH_TAC THEN POP_ASSUM(MATCH_MP_TAC o ONCE_REWRITE_RULE [MONO_NOT_EQ]) THEN
     ASM_SIMP_TAC arith_ss [],
-    MP_TAC(ISPECL [``f:num->num``, ``((0:num)..n)``] UPPER_BOUND_FINITE_SET) THEN
+    MP_TAC(ISPECL [``f:num->num``, ``{ 0n..n}``] UPPER_BOUND_FINITE_SET) THEN
     REWRITE_TAC[FINITE_NUMSEG, IN_NUMSEG, ZERO_LESS_EQ] THEN
     DISCH_THEN(X_CHOOSE_TAC ``p:num``) THEN
     EXISTS_TAC
-     ``sum(IMAGE (f:num->num) s INTER (N..p)) (\i. abs(x i :real))`` THEN
+     ``sum(IMAGE (f:num->num) s INTER {N..p}) (\i. abs(x i :real))`` THEN
     CONJ_TAC THENL [ALL_TAC,
      MATCH_MP_TAC (REAL_ARITH ``abs x < y ==> x < y:real``) THEN
      ASM_SIMP_TAC real_ss []] THEN MATCH_MP_TAC SUM_SUBSET_SIMPLE THEN
@@ -18629,7 +18629,7 @@ val BANACH_FIX = store_thm ("BANACH_FIX",
    [INDUCT_TAC THEN ASM_SIMP_TAC std_ss [] THEN
     METIS_TAC[MEMBER_NOT_EMPTY, SUBSET_DEF, IN_IMAGE],
     ALL_TAC] THEN
-  UNDISCH_THEN ``z (0:num) = @x:real. x IN s`` (K ALL_TAC) THEN
+  UNDISCH_THEN ``z  0n = @x:real. x IN s`` (K ALL_TAC) THEN
   SUBGOAL_THEN ``?x:real. x IN s /\ (z --> x) sequentially`` MP_TAC THENL
    [ALL_TAC,
     DISCH_THEN (X_CHOOSE_TAC ``a:real``) THEN EXISTS_TAC ``a:real`` THEN
@@ -18662,7 +18662,7 @@ val BANACH_FIX = store_thm ("BANACH_FIX",
     ALL_TAC] THEN
   SUBGOAL_THEN
    ``!m n:num. (&1 - c) * dist(z(m):real,z(m+n))
-                <= c pow m * dist(z(0),z(1:num)) * (&1 - c pow n)``
+                <= c pow m * dist(z(0),z 1n) * (&1 - c pow n)``
   ASSUME_TAC THENL
    [GEN_TAC THEN INDUCT_TAC THENL
      [REWRITE_TAC[ADD_CLAUSES, DIST_REFL, REAL_MUL_RZERO, GSYM REAL_MUL_ASSOC] THEN
